formalization/MailboxActors/MailboxActors/Examples/Anoma/Identity/NameRegistry/Behaviour.lean
@@ -66,8 +66,7 @@ def nameRegistrySubmitAction
   Effect.update { env with
     localState := { st with registrationCount := st.registrationCount + 1 } }
 
-def nameRegistryActions
-    : @Behaviour (S A) AnomaIdx.nameRegistry :=
+def nameRegistryActions : @Behaviour (S A) AnomaIdx.nameRegistry :=
   letI := S A
   [ { Witness := A.ExternalIdentity
       guard := nameRegistryQueryGuard A
@@ -76,15 +75,13 @@ def nameRegistryActions
       guard := nameRegistrySubmitGuard A
       action := nameRegistrySubmitAction A } ]
 
-private
-theorem nameRegistryNonOverlapping
-    : @NonOverlappingGuards (S A) _ (nameRegistryActions A) := by
+private theorem nameRegistryNonOverlapping :
+    @NonOverlappingGuards (S A) _ (nameRegistryActions A) := by
   letI := S A; intro inp
   simp only [nameRegistryActions, List.filter]
   cases h : @GuardInput.msg (S A) _ inp <;> simp_all
 
-def nameRegistryBehaviour
-    : @WellFormedBehaviour (S A) AnomaIdx.nameRegistry :=
+def nameRegistryBehaviour : @WellFormedBehaviour (S A) AnomaIdx.nameRegistry :=
   letI := S A
   { actions := nameRegistryActions A
     nonOverlapping := nameRegistryNonOverlapping A }
