formalization/MailboxActors/MailboxActors/Examples/Anoma/Identity/ReadDeleg/Behaviour.lean
@@ -66,8 +66,7 @@ def readDelegSubmitAction
   Effect.update { env with
     localState := { st with evidenceCount := st.evidenceCount + 1 } }
 
-def readDelegActions
-    : @Behaviour (S A) AnomaIdx.readDeleg :=
+def readDelegActions : @Behaviour (S A) AnomaIdx.readDeleg :=
   letI := S A
   [ { Witness := A.ExternalIdentity
       guard := readDelegQueryGuard A
@@ -76,15 +75,13 @@ def readDelegActions
       guard := readDelegSubmitGuard A
       action := readDelegSubmitAction A } ]
 
-private
-theorem readDelegNonOverlapping
-    : @NonOverlappingGuards (S A) _ (readDelegActions A) := by
+private theorem readDelegNonOverlapping :
+    @NonOverlappingGuards (S A) _ (readDelegActions A) := by
   letI := S A; intro inp
   simp only [readDelegActions, List.filter]
   cases h : @GuardInput.msg (S A) _ inp <;> simp_all
 
-def readDelegBehaviour
-    : @WellFormedBehaviour (S A) AnomaIdx.readDeleg :=
+def readDelegBehaviour : @WellFormedBehaviour (S A) AnomaIdx.readDeleg :=
   letI := S A
   { actions := readDelegActions A
     nonOverlapping := readDelegNonOverlapping A }
