formalization/MailboxActors/MailboxActors/Examples/Anoma/Identity/SignDeleg/Behaviour.lean
@@ -66,8 +66,7 @@ def signDelegSubmitAction
   Effect.update { env with
     localState := { st with evidenceCount := st.evidenceCount + 1 } }
 
-def signDelegActions
-    : @Behaviour (S A) AnomaIdx.signDeleg :=
+def signDelegActions : @Behaviour (S A) AnomaIdx.signDeleg :=
   letI := S A
   [ { Witness := A.ExternalIdentity
       guard := signDelegQueryGuard A
@@ -76,15 +75,13 @@ def signDelegActions
       guard := signDelegSubmitGuard A
       action := signDelegSubmitAction A } ]
 
-private
-theorem signDelegNonOverlapping
-    : @NonOverlappingGuards (S A) _ (signDelegActions A) := by
+private theorem signDelegNonOverlapping :
+    @NonOverlappingGuards (S A) _ (signDelegActions A) := by
   letI := S A; intro inp
   simp only [signDelegActions, List.filter]
   cases h : @GuardInput.msg (S A) _ inp <;> simp_all
 
-def signDelegBehaviour
-    : @WellFormedBehaviour (S A) AnomaIdx.signDeleg :=
+def signDelegBehaviour : @WellFormedBehaviour (S A) AnomaIdx.signDeleg :=
   letI := S A
   { actions := signDelegActions A
     nonOverlapping := signDelegNonOverlapping A }
