formalization/MailboxActors/MailboxActors/Examples/Anoma/Identity/Verification/Behaviour.lean
@@ -53,22 +53,19 @@ def verificationAction
   let result := A.verify_ backend eid signable sig
   Effect.send AnomaIdx.identity replyTo (.verifyResult result)
 
-def verificationActions
-    : @Behaviour (S A) AnomaIdx.verification :=
+def verificationActions : @Behaviour (S A) AnomaIdx.verification :=
   letI := S A
   [ { Witness := A.ExternalIdentity × A.Signable × A.Signature × Bool × Address
       guard := verificationGuard A
       action := verificationAction A } ]
 
-private
-theorem verificationNonOverlapping
-    : @NonOverlappingGuards (S A) _ (verificationActions A) := by
+private theorem verificationNonOverlapping :
+    @NonOverlappingGuards (S A) _ (verificationActions A) := by
   letI := S A; intro inp
   simp only [verificationActions, List.filter]
   split <;> simp
 
-def verificationBehaviour
-    : @WellFormedBehaviour (S A) AnomaIdx.verification :=
+def verificationBehaviour : @WellFormedBehaviour (S A) AnomaIdx.verification :=
   letI := S A
   { actions := verificationActions A
     nonOverlapping := verificationNonOverlapping A }
