formalization/MailboxActors/MailboxActors/Examples/Anoma/Infra/Logging/Behaviour.lean
@@ -34,22 +34,19 @@ def loggingAppendAction
     localState := { entries := env.localState.entries ++ [w]
                     position := env.localState.position + 1 } }
 
-def loggingActions
-    : @Behaviour (S A) AnomaIdx.logging :=
+def loggingActions : @Behaviour (S A) AnomaIdx.logging :=
   letI := S A
   [ { Witness := String
       guard := loggingAppendGuard A
       action := loggingAppendAction A } ]
 
-private
-theorem loggingNonOverlapping
-    : @NonOverlappingGuards (S A) _ (loggingActions A) := by
+private theorem loggingNonOverlapping :
+    @NonOverlappingGuards (S A) _ (loggingActions A) := by
   letI := S A; intro inp
   simp only [loggingActions, List.filter]
   split <;> simp
 
-def loggingBehaviour
-    : @WellFormedBehaviour (S A) AnomaIdx.logging :=
+def loggingBehaviour : @WellFormedBehaviour (S A) AnomaIdx.logging :=
   letI := S A
   { actions := loggingActions A
     nonOverlapping := loggingNonOverlapping A }
